verif/verif_isnodeparent.v
@@ -1,0 +1,58 @@
+(** * verif_isnodeparent.v : Correctness proof of isNodeParent *)
+
+Require Import VST.floyd.proofauto.
+Require Import VST.floyd.library.
+Require Import relation_mem.
+Instance CompSpecs : compspecs. make_compspecs prog. Defined.
+Definition Vprog : varspecs. mk_varspecs prog. Defined.
+
+Require Import VST.msl.wand_frame.
+Require Import VST.msl.iter_sepcon.
+Require Import VST.floyd.reassoc_seq.
+Require Import VST.floyd.field_at_wand.
+Require Import FunInd.
+Require Import btrees.
+Require Import index.
+Require Import btrees_sep.
+Require Import btrees_spec.
+Require Import verif_findindex.
+
+Lemma body_isNodeParent: semax_body Vprog Gprog f_isNodeParent isNodeParent_spec.
+Proof.
+  start_function.
+  forward_call(n,key).
+  forward_if(PROP() LOCAL(temp _t'2 (Val.of_bool (negb (isNodeParent n key))); temp _idx (rep_index (findChildIndex n key)); temp _node (getval n); temp _key (Vint (Int.repr key))) SEP (btnode_rep n)).
+  - forward.                    (* t'2=1 *)
+    entailer!.
+    destruct (findChildIndex n key) eqn:FCI.
+    unfold isNodeParent. rewrite FCI. simpl. auto.
+    inv H1. admit.              (* contradiction in h6 *)
+  - destruct n as [ptr0 le isLeaf First Last pn].
+    pose (n:=btnode val ptr0 le isLeaf First Last pn).
+    rewrite unfold_btnode_rep. simpl. Intros.
+    forward.                    (* t'3=node->numKeys *)
+    forward.                    (* t'2= (idx==t'3-1) *)
+    + admit.                    (* tc_expr *)
+    + gather_SEP 0 1 2 3. replace_SEP 0 (btnode_rep n).
+      { entailer!. }
+      entailer!.
+      unfold isNodeParent. fold n.
+      destruct (findChildIndex n key) eqn:FCI.
+      { unfold findChildIndex, n in FCI. rewrite FCI in H1. simpl in H1. inv H1. }
+      rewrite negb_involutive.
+      destruct (S n0 =? numKeys n)%nat eqn:Hnum.
+      * unfold findChildIndex, n in FCI. rewrite FCI.
+        simpl.
+        inv Hnum. destruct (numKeys_le le); inv H8.
+        assert (Z.of_nat (S n1) -1 = Z.of_nat n1) by admit.
+        rewrite H7. admit.      (* true from H9 *)
+      * simpl. unfold findChildIndex, n in FCI. rewrite FCI.
+        simpl.
+        admit.                  (* ok from Hnum *)
+  - forward_if.
+    + forward.                  (* return *)
+      rewrite H1. entailer!.
+    + forward.                  (* skip *)
+      forward.                  (* return *)
+      rewrite H1. entailer!.
+Admitted.
